Make signatures monomorphic; simplify polyf.

theories/generic.v
@@ -147,6 +147,57 @@ Proof.
 elim: n i=> [|n IH] // [i|] //=; by rewrite IH.
 Qed.
 
+Section Ilist.
+
+Variables (T : Type).
+
+Definition ilist n := iter n (prod T) unit.
+
+Fixpoint nth_ilist n : ilist n -> fin n -> T :=
+  match n with
+  | 0    => fun l i => match i with end
+  | n.+1 => fun l i => if i is Some j then nth_ilist l.2 j else l.1
+  end.
+
+Fixpoint ilist_of_seq s : ilist (size s) :=
+  match s with
+  | [::] => tt
+  | x :: s => (x, ilist_of_seq s)
+  end.
+
+Fixpoint seq_of_ilist n : ilist n -> seq T :=
+  match n with
+  | 0    => fun l => [::]
+  | n.+1 => fun l => l.1 :: seq_of_ilist l.2
+  end.
+
+End Ilist.
+
+Fixpoint imap T S (f : T -> S) n : ilist T n -> ilist S n :=
+  match n with
+  | 0    => fun l => tt
+  | n.+1 => fun l => (f l.1, imap f l.2)
+  end.
+
+Lemma imap_eq (T S : Type) (f g : T -> S) :
+  f =1 g ->
+  forall n, @imap _ _ f n =1 @imap _ _ g n.
+Proof.
+by move=> efg; elim=> [[]|n IH] // [x l] /=; rewrite efg IH.
+Qed.
+
+Lemma imap1 (T: Type) n (l : ilist T n) : imap id l = l.
+Proof.
+by elim: n l=> /= [[]|n IH] // [x l] /=; rewrite IH.
+Qed.
+
+Lemma imap_comp (T S R : Type)
+                (f : T -> S) (g : S -> R) n (l : ilist T n) :
+  imap g (imap f l) = imap (g \o f) l.
+Proof.
+by elim: n l=> [[]|n IH] //= [x l] /=; rewrite IH.
+Qed.
+
 Section Hlist.
 
 Variables (I : Type) (T_ : I -> Type).
@@ -296,91 +347,81 @@ Fixpoint hfun_eq I (T_ S_ : I -> Type) (e : forall i, T_ i = S_ i) ix R :
   | i :: ix => f_equal2 (fun X Y => X -> Y) (e i) (hfun_eq e ix R)
   end.
 
-Variant kind T := Other of T | Rec.
-
-Arguments Rec {_}.
-
-Definition kmap T S (f : T -> S) (k : kind T) :=
-  if k is Other x then Other (f x) else Rec.
-Definition arity T := seq (kind T).
-Definition signature T := seq (arity T).
-Definition sig_map T S (f : T -> S) (s : signature T) : signature S :=
-  [seq [seq kmap f k | k <- a] | a <- s].
-
 Section PolyFunctor.
 
-Variables (A : Type) (A_sort : A -> Type).
+Variables (n : nat) (A : fin n -> Type) (ns : fin n -> nat).
 
-Local Coercion A_sort : A >-> Sortclass.
+Record polyf T := Polyf {
+  pconstr : fin n;
+  pargs   : A pconstr;
+  prargs  : ilist T (ns pconstr)
+}.
 
-Implicit Types (k : kind A) (a : arity A).
+Definition poly_fmap T S (f : T -> S) (x : polyf T) : polyf S :=
+  Polyf (pargs x) (imap f (prargs x)).
 
-Variable s : signature A.
+Lemma poly_fmap_eq S R (f g : S -> R) :
+  f =1 g ->
+  poly_fmap f =1 poly_fmap g.
+Proof.
+move=> efg [c args rargs] /=; rewrite /poly_fmap /=; congr Polyf.
+exact/imap_eq.
+Qed.
 
-Definition type_of_arg S (k : kind A) : Type :=
+Lemma poly_fmap1 S (x : polyf S) : poly_fmap id x = x.
+Proof.
+rewrite /poly_fmap; case: x=> i args rargs /=; by rewrite imap1.
+Qed.
+
+Lemma poly_fmap_comp T S R f (g : S -> R) (x : polyf T) :
+  poly_fmap (g \o f) x = poly_fmap g (poly_fmap f x).
+Proof.
+by case: x=> [i args rargs]; rewrite /poly_fmap /= imap_comp.
+Qed.
+
+Canonical polyf_functor :=
+  Functor poly_fmap_eq poly_fmap1 poly_fmap_comp.
+
+Lemma Polyf_inj T i a1 r1 a2 r2 :
+  @Polyf T i a1 r1 = @Polyf _ i a2 r2 -> (a1, r1) = (a2, r2).
+Proof.
+pose get x :=
+  if leq_fin (pconstr x) i is inl e then
+    cast (fun k : fin n => A k * ilist T (ns k))%type
+         e (pargs x, prargs x)
+  else (a1, r1).
+by move=> /(f_equal get); rewrite /get /= leq_finii /=.
+Qed.
+
+End PolyFunctor.
+
+Arguments Polyf {_ _ _ _} _ _ _.
+
+Variant kind := Other of Type | Rec.
+
+Definition is_other k := if k is Other R then Some R else None.
+Definition is_rec k := ~~ (is_other k).
+
+Module CoqInd.
+
+Section Basic.
+
+Variable (T : Type).
+
+Definition arity := seq kind.
+Definition signature := seq arity.
+
+Implicit Types (k : kind) (a : arity) (s : signature).
+
+Definition type_of_arg S (k : kind) : Type :=
   if k is Other R then R else S.
 
 Definition type_of_arg_map S R (f : S -> R) k :
   type_of_arg S k -> type_of_arg R k :=
   if k is Rec then f else id.
 
-Record polyf T := Polyf {
-  pconstr : fin (size s);
-  pargs : hlist (type_of_arg T) (nth_fin pconstr)
-}.
-
-Definition poly_fmap S R (f : S -> R) (x : polyf S) : polyf R :=
-  Polyf (hmap (type_of_arg_map f) (pargs x)).
-
-Lemma poly_fmap_eq S R (f g : S -> R) :
-  f =1 g ->
-  poly_fmap f =1 poly_fmap g.
-Proof.
-move=> efg [c args] /=; rewrite /poly_fmap /=; congr Polyf.
-by apply/hmap_eq; case.
-Qed.
-
-Lemma poly_fmap1 S (x : polyf S) : poly_fmap id x = x.
-Proof.
-rewrite /poly_fmap; case: x=> i args /=.
-rewrite (_ : hmap _ args = hmap (fun _ => id) args) ?hmap1 //.
-by elim: (nth_fin i) args=> {i} [[]|[R|] ks IH] //= [arg args] /=;
-rewrite IH.
-Qed.
-
-Lemma poly_fmap_comp T S R f (g : S -> R) (x : polyf T) :
-  poly_fmap (g \o f) x = poly_fmap g (poly_fmap f x).
-Proof.
-case: x=> [i args]; rewrite /poly_fmap /= hmap_comp; congr Polyf.
-by apply/hmap_eq; case=> [?|].
-Qed.
-
-Canonical polyf_functor :=
-  Functor poly_fmap_eq poly_fmap1 poly_fmap_comp.
-
-Lemma Polyf_inj T i : injective (@Polyf T i).
-Proof.
-move=> args1 args2 e.
-pose get x :=
-  (if leq_fin (pconstr x) i is inl e then
-     cast (fun i => hlist (type_of_arg T) (nth_fin i)) e (pargs x)
-   else args1).
-move/(f_equal get): e; by rewrite /get leq_finii.
-Qed.
-
-End PolyFunctor.
-
-Module CoqInd.
-
-Section Basic.
-
-Variable (A : Type) (A_sort : A -> Type) (T : Type).
-Local Coercion A_sort : A >-> Sortclass.
-
-Implicit Types (k : kind A) (a : arity A) (s : signature A).
-
 Definition constructors s :=
-  hlist (fun a => hfun (type_of_arg A_sort T) a T) s.
+  hlist (fun a => hfun (type_of_arg T) a T) s.
 
 Fixpoint branch S a : Type :=
   match a with
@@ -392,7 +433,7 @@ Fixpoint branch S a : Type :=
 Definition recursor s := forall S, hfun (branch S) s (T -> S).
 
 Fixpoint branch_of_hfun S a :
-  hfun (type_of_arg A_sort (T * S)) a S -> branch S a :=
+  hfun (type_of_arg (T * S)) a S -> branch S a :=
   match a with
   | Other R :: a => fun f x   => branch_of_hfun (f x)
   | Rec     :: a => fun f x y => branch_of_hfun (f (x, y))
@@ -400,7 +441,7 @@ Fixpoint branch_of_hfun S a :
   end.
 
 Fixpoint hfun_of_branch S a :
-  branch S a -> hfun (type_of_arg A_sort (T * S)) a S :=
+  branch S a -> hfun (type_of_arg (T * S)) a S :=
   match a with
   | Other R :: a => fun f x => hfun_of_branch (f x)
   | Rec     :: a => fun f p => hfun_of_branch (f p.1 p.2)
@@ -417,23 +458,23 @@ Definition recursor_eq s (cs : constructors s) (r : recursor s) :=
   forall S,
   all_hlist (fun bs : hlist (branch S) s =>
   all_fin   (fun i : fin (size s) =>
-  all_hlist (fun args : hlist (type_of_arg A_sort T) (nth_fin i) =>
+  all_hlist (fun args : hlist (type_of_arg T) (nth_fin i) =>
     r S bs (nth_hlist cs i args) =
     hfun_of_branch (nth_hlist bs i)
                    (hmap (type_of_arg_map (fun x => (x, r S bs x))) args)))).
 
 Definition destructor s :=
-  forall S, hfun (fun a => hfun (type_of_arg A_sort T) a S) s (T -> S).
+  forall S, hfun (fun a => hfun (type_of_arg T) a S) s (T -> S).
 
 Definition destructor_eq s (cs : constructors s) (d : destructor s) :=
   forall S,
-  all_hlist (fun bs : hlist (fun ks => hfun (type_of_arg A_sort T) ks S) s =>
+  all_hlist (fun bs : hlist (fun ks => hfun (type_of_arg T) ks S) s =>
   all_fin   (fun i : fin (size s) =>
-  all_hlist (fun args : hlist (type_of_arg A_sort T) (nth_fin i) =>
+  all_hlist (fun args : hlist (type_of_arg T) (nth_fin i) =>
     d S bs (nth_hlist cs i args) = nth_hlist bs i args))).
 
 Fixpoint ind_branch (P : T -> Type) a :
-  hfun (type_of_arg A_sort T) a T -> Type :=
+  hfun (type_of_arg T) a T -> Type :=
   match a with
   | Other R :: a => fun c => forall x : R,        ind_branch P (c x)
   | Rec     :: a => fun c => forall x : T, P x -> ind_branch P (c x)
@@ -450,12 +491,12 @@ End Basic.
 
 Section ClassDef.
 
-Variables (A : Type) (A_sort : A -> Type) (s : signature A).
+Variables (s : signature).
 
 Record mixin_of T := Mixin {
-  Cons      : constructors A_sort T s;
-  rec       : recursor A_sort T s;
-  case      : destructor A_sort T s;
+  Cons      : constructors T s;
+  rec       : recursor T s;
+  case      : destructor T s;
   _         : recursor_eq Cons rec;
   _         : destructor_eq Cons case;
   _         : forall P, ind_at P Cons;
@@ -478,7 +519,7 @@ Module Exports.
 Coercion sort : type >-> Sortclass.
 Coercion class : type >-> mixin_of.
 Notation coqIndType := type.
-Notation CoqIndType A A_sort s T m := (@Pack A A_sort s T m T).
+Notation CoqIndType s T m := (@Pack s T m T).
 Notation CoqIndMixin := Mixin.
 End Exports.
 
@@ -487,44 +528,115 @@ Export CoqInd.Exports.
 
 Section CoqIndTheory.
 
-Variables (A : Type) (A_sort : A -> Type) (s : signature A).
-Variable T : coqIndType A_sort s.
+Import CoqInd.
 
-Local Notation F := (polyf_functor A_sort s).
+Variables (s : signature).
+Variable T : coqIndType s.
+
+Fixpoint args_of_arity a : Type :=
+  match a with
+  | Other R :: a => R * args_of_arity a
+  | Rec     :: a => args_of_arity a
+  | [::]         => unit
+  end.
+
+Fixpoint rargs_of_arity a : Type :=
+  match a with
+  | Other R :: a => args_of_arity a
+  | Rec     :: a => T * args_of_arity a
+  | [::]         => unit
+  end.
+
+Fixpoint proj_args S a : hlist (type_of_arg S) a -> args_of_arity a :=
+  match a with
+  | Other R :: a => fun l => (l.1, proj_args l.2)
+  | Rec     :: a => fun l => proj_args l.2
+  | [::]         => fun l => l
+  end.
+
+Fixpoint proj_rargs S a : hlist (type_of_arg S) a -> ilist S (count is_rec a) :=
+  match a with
+  | Other R :: a => fun l => proj_rargs l.2
+  | Rec     :: a => fun l => (l.1, proj_rargs l.2)
+  | [::]         => fun l => l
+  end.
+
+Fixpoint pack_args S a : args_of_arity a -> ilist S (count is_rec a) -> hlist (type_of_arg S) a :=
+  match a with
+  | Other R :: a => fun args rargs => (args.1, @pack_args S a args.2 rargs)
+  | Rec     :: a => fun args rargs => (rargs.1, @pack_args S a args rargs.2)
+  | [::]         => fun args rargs => tt
+  end.
+
+Lemma proj_args_pack S a args rargs :
+  proj_args (@pack_args S a args rargs) = args.
+Proof.
+elim: a args rargs=> [[]|[R|] a IH] //=.
+by case=> [??] ?; rewrite IH.
+Qed.
+
+Lemma proj_rargs_pack S a args rargs :
+  proj_rargs (@pack_args S a args rargs) = rargs.
+Proof.
+elim: a args rargs=> [_ []|[R|] a IH] //=.
+by move=> ? [??]; rewrite IH.
+Qed.
+
+Lemma hmap_pack S R (f : S -> R) a args rargs :
+  hmap (type_of_arg_map f) (@pack_args _ a args rargs) =
+  pack_args args (imap f rargs).
+Proof.
+elim: a args rargs=> [|[?|] a IH] //=.
+- by move=> [??] ?; rewrite IH.
+- by move=> ? [??]; rewrite IH.
+Qed.
+
+Let F :=
+  (@polyf_functor (size s)
+                  (fun k => args_of_arity (nth_fin k))
+                  (fun k => count is_rec (nth_fin k))).
 
 Definition coqInd_Roll (x : F T) :=
-  nth_hlist (@CoqInd.Cons _ _ _ _ T) (pconstr x) (pargs x).
+  nth_hlist (@Cons _ _ T) (pconstr x) (pack_args (pargs x) (prargs x)).
 
-Definition branches_of_hfun S (body : F (T * S)%type -> S) :=
-  hlist_of_fun (fun i => CoqInd.branch_of_hfun (hcurry (fun l => body (Polyf l)))).
+Definition branches_of_fun S (body : F (T * S)%type -> S) :=
+  hlist_of_fun (fun i =>
+    branch_of_hfun
+      (hcurry
+         (fun l => body (Polyf i (proj_args l) (proj_rargs l))))).
 
 Definition coqInd_rec S (body : F (T * S)%type -> S) :=
-  happ (@CoqInd.rec _ _ _ _ T S) (branches_of_hfun body).
+  happ (@CoqInd.rec _ _ T S) (branches_of_fun body).
 
 Definition coqInd_case S (body : F T -> S) :=
-  happ (@CoqInd.case _ _ _ _ T S)
-       (hlist_of_fun (fun i => hcurry (fun l => body (Polyf l)))).
+  happ (@CoqInd.case _ _ T S)
+       (hlist_of_fun
+          (fun i =>
+             hcurry
+               (fun l =>
+                  body (Polyf i (proj_args l) (proj_rargs l))))).
 
 Lemma coqInd_recE S f a : @coqInd_rec S f (coqInd_Roll a) =
                           f (fmap (fun x => (x, coqInd_rec f x)) a).
 Proof.
-case: a=> [i args]; have := CoqInd.recE T S.
-move/all_hlistP/(_ (branches_of_hfun f)).
+case: a=> [i args rargs]; have := CoqInd.recE T S.
+move/all_hlistP/(_ (branches_of_fun f)).
 move/all_finP/(_ i).
-move/all_hlistP/(_ args).
+move/all_hlistP/(_ (pack_args args rargs)).
 rewrite /coqInd_rec /coqInd_Roll => -> /=.
-rewrite /poly_fmap /=; move: (hmap _ _)=> l.
-by rewrite /branches_of_hfun nth_hlist_of_fun CoqInd.branch_of_hfunK hcurryK.
+rewrite /poly_fmap /= nth_hlist_of_fun branch_of_hfunK hcurryK.
+by rewrite !hmap_pack proj_args_pack proj_rargs_pack.
 Qed.
 
 Lemma coqInd_caseE S f a : coqInd_case f (coqInd_Roll a) = f a :> S.
 Proof.
-case: a => [i args]; have := CoqInd.caseE T S.
-move/all_hlistP/(_ (hlist_of_fun (fun i => hcurry (fun l => f (Polyf l))))).
+case: a => [i args rargs]; have := CoqInd.caseE T S.
+move/all_hlistP.
+move/(_ (hlist_of_fun (fun i => hcurry (fun l => f (Polyf i (proj_args l) (proj_rargs l)))))).
 move/all_finP/(_ i).
-move/all_hlistP/(_ args).
+move/all_hlistP/(_ (pack_args args rargs)).
 rewrite /coqInd_case /coqInd_Roll => -> /=.
-by rewrite nth_hlist_of_fun hcurryK.
+by rewrite nth_hlist_of_fun hcurryK proj_args_pack proj_rargs_pack.
 Qed.
 
 Lemma coqInd_indP P :
@@ -542,15 +654,17 @@ have {indP} indP:
   exact: (hyps (Some i)).
 move=> hyps; apply: indP=> j.
 have {hyps} hyps:
-  forall args : hlist (type_of_arg _ {x : S & P x}) (nth_fin j),
-    P (nth_hlist Cons j (hmap (type_of_arg_map tag) args)).
-  move=> args; exact: (hyps (Polyf args)).
+  forall (args : args_of_arity (nth_fin j))
+         (rargs : ilist {x & P x} (count is_rec (nth_fin j))),
+    P (nth_hlist Cons j (hmap (type_of_arg_map tag) (pack_args args rargs))).
+  move=> args rargs.
+  move: (hyps (Polyf j args rargs)); by rewrite hmap_pack.
 elim: (nth_fin j) (nth_hlist Cons j) hyps=> [|[i|] ks IH] //=.
-- by move=> ? /(_ tt).
+- by move=> ? /(_ tt tt).
 - move=> c hyps x; apply: IH=> args.
   exact: (hyps (x, args)).
-- move=> constr hyps x H; apply: IH=> args.
-  exact: (hyps (existT _ x H, args)).
+- move=> constr hyps x H; apply: IH=> args rargs.
+  exact: (hyps args (existT _ x H, rargs)).
 Qed.
 
 Definition coqInd_indMixin :=
@@ -560,159 +674,81 @@ Canonical coqInd_indType :=
 
 End CoqIndTheory.
 
-(*
-Section CoqIndTransport.
-
-Variables (A : Type) (A_sort : A -> Type).
-Variables (B : Type) (A_of_B : B -> A).
-
-Fixpoint branch_mapA T S a :
-   CoqInd.branch A_sort T S [seq kmap A_of_B k | k <- a] =
-   CoqInd.branch (A_sort \o A_of_B) T S a :=
-  match a with
-  | [::] => erefl
-  | Other R :: a => f_equal (fun U => A_sort (A_of_B R) -> U) (branch_mapA T S a)
-  | Rec     :: a => f_equal (fun U => T -> S -> U) (branch_mapA T S a)
-  end.
-
-Definition type_of_arg_mapA T k :
-  type_of_arg A_sort T (kmap A_of_B k) = type_of_arg (A_sort \o A_of_B) T k :=
-  match k with
-  | Rec => erefl
-  | Other R => erefl
-  end.
-
-Fixpoint constructors_mapA T s :
-  CoqInd.constructors A_sort T (sig_map A_of_B s) =
-  CoqInd.constructors (A_sort \o A_of_B) T s :=
-  match s with
-  | [::] => erefl
-  | a :: s =>
-    let e := etrans (hfun_map (type_of_arg A_sort T) (kmap A_of_B) T a)
-                    (hfun_eq (type_of_arg_mapA T) a T) in
-    f_equal2 prod e (constructors_mapA T s)
-  end.
-
-Definition recursor_mapA T s :
-  CoqInd.recursor A_sort T (sig_map A_of_B s) ->
-  CoqInd.recursor (A_sort \o A_of_B) T s :=
-  fun rec S =>
-    let e := etrans (hfun_map (CoqInd.branch A_sort T S) _ (T -> S) s)
-                    (hfun_eq (branch_mapA T S) s (T -> S)) in
-    cast id e (rec S).
-
-Definition destructor_mapA T s :
-  CoqInd.destructor A_sort T (sig_map A_of_B s) ->
-  CoqInd.destructor (A_sort \o A_of_B) T s.
-move=> case S.
-pose e1 := hfun_map (fun a => hfun (type_of_arg A_sort T) a S) (map (kmap A_of_B)) (T -> S) s.
-pose e2 := hfun_eq (fun a => hfun_map (type_of_arg A_sort T) (kmap A_of_B) S a) s (T -> S).
-pose e3 := hfun_eq (fun a => hfun_eq (type_of_arg_mapA T) a S) s (T -> S).
-pose e := etrans e1 (etrans e2 e3).
-exact: (cast id e (case S)).
-Defined.
-
-Lemma recursion_eqP T s Cons rec:
-  @CoqInd.recursor_eq _ _ T (sig_map A_of_B s) Cons rec ->
-  @CoqInd.recursor_eq _ _ T s
-                      (cast id (constructors_mapA T s) Cons)
-                      (recursor_mapA rec).
-Proof.
-move=> recE S.
-apply/all_hlistP=> l.
-apply/all_finP=> i.
-apply/all_hlistP=> args.
-move/(_ S)/all_hlistP: recE.
-pose el := etrans (hlist_map (CoqInd.branch A_sort T S) (map (kmap A_of_B)) s)
-                  (hlist_eq (branch_mapA T S) s).
-move/(_ (cast id (esym el) l))/all_finP.
-move
-
-
-
-Variables (T : coqIndType A_sort (sig_map A_of_B s)).
-*)
-
-Module CoqIndEqType.
+Module IndEqType.
 
 Section ClassDef.
 
-Record class_of A A_sort s T := Class {
+Record class_of T F := Class {
   base : Equality.class_of T;
-  mixin : @CoqInd.mixin_of A A_sort s T
+  mixin : Ind.mixin_of T F
 }.
 
-Record type A A_sort s :=
-  Pack {sort : Type; _ : @class_of A A_sort s sort; _ : Type}.
+Record type F :=
+  Pack {sort : Type; _ : class_of sort F; _ : Type}.
 Local Coercion sort : type >-> Sortclass.
 
-Variables (A : Type) (A_sort : A -> Type) (s : signature A).
-Variables (T : Type) (cT : type A_sort s).
+Variables (F : functor) (T : Type) (cT : type F).
 Definition class :=
-  let: Pack _ c _ as cT' := cT return class_of A_sort s cT' in c.
-Definition clone c of phant_id class c := @Pack _ A_sort s T c T.
+  let: Pack _ c _ as cT' := cT return class_of cT' F in c.
+Definition clone c of phant_id class c := @Pack F T c T.
 Let xT := let: Pack T _ _ := cT in T.
-Notation xclass := (class : class_of A_sort s xT).
+Notation xclass := (class : class_of xT F).
 
-Definition pack c := @Pack _ A_sort s T c T.
+Definition pack c := @Pack F T c T.
 
 Definition eqType := @Equality.Pack cT (base xclass) xT.
-Definition coqIndType := @CoqInd.Pack A A_sort s cT (mixin xclass) xT.
+Definition indType := @Ind.Pack F cT (mixin xclass) xT.
 
 End ClassDef.
 
 Section Exports.
 Coercion sort : type >-> Sortclass.
 Coercion eqType : type >-> Equality.type.
-Coercion coqIndType : type >-> CoqInd.type.
-Notation coqIndEqType := type.
+Coercion indType : type >-> Ind.type.
+Notation indEqType := type.
 End Exports.
 
-End CoqIndEqType.
+End IndEqType.
 
 Section GenericEqType.
 
-Variable (A : Type) (A_sort : A -> eqType) (s : signature A).
-Variable (T : coqIndType A_sort s).
+Variable (s : seq (eqType * nat)).
+Let F := (@polyf_functor (size s)
+                         (fun i => (nth_fin i).1)
+                         (fun i => (nth_fin i).2)).
+Variable (T : indType F).
 
 Definition ind_eq : T -> T -> bool :=
   rec (fun args1 x2 =>
          let args2 := unroll x2 in
          match leq_fin (pconstr args2) (pconstr args1) with
          | inl e =>
-           hfold (fun k =>
-                    if k is Other i then
-                      fun args res => (args.1 == args.2) && res
-                    else
-                      fun args res =>
-                        (args.1.2 args.2) && res)
-                 true
-                 (hzip (pargs args1)
-                       (cast (fun i => hlist (type_of_arg _ T) (nth_fin i))
-                             e (pargs args2)))
+           (pargs args1 == (cast _ e (pargs args2))) &&
+           all id [seq p.1.2 p.2
+                  | p <- zip (seq_of_ilist (prargs args1))
+                             (seq_of_ilist (prargs args2))]
          | inr _ => false
          end).
 
 Lemma ind_eqP : Equality.axiom ind_eq.
 Proof.
-elim/indP=> [[i_x x]] y.
-rewrite /ind_eq recE /= -[rec _]/(ind_eq).
-rewrite -{1}[y]unrollK; move: {y} (unroll y)=> [i_y y] /=.
+elim/indP=> [[i_x xargs x]] y.
+rewrite /ind_eq recE /= -[rec _]/(ind_eq) /poly_fmap /=.
+rewrite -{1}[y]unrollK; move: {y} (unroll y)=> [i_y yargs y] /=.
 case le: (leq_fin i_y i_x)=> [e|b]; last first.
-  constructor=> /Roll_inj /= [] e _.
+  constructor=> /Roll_inj /= [] e _ _.
   by move: le; rewrite e leq_finii.
-case: i_x / e x {le} => /= x.
-apply/(@iffP (hmap (type_of_arg_map tag) x = y)); first last.
-- by move=> /Roll_inj/Polyf_inj.
-- by move=> <-.
-elim: {i_y} (nth_fin i_y) x y=> [|[R|] ks IH] //=.
-- by move=> [] []; constructor.
-- move=> [x xs] [y ys] /=; apply/(iffP andP).
-  + by case=> [/eqP -> /IH ->].
-  + by case=> [<- <-]; split=> //; apply/IH.
-- move=> [[x IHx] xs] [y ys] /=; apply(iffP andP).
-  + by case=> [/IHx -> /IH ->].
-  + by case=> [<- <-]; split; [apply/IHx| apply/IH].
+case: i_x / e xargs x {le} => /= xargs x.
+apply/(@iffP (xargs = yargs /\ imap tag x = y)); first last.
+- by move=> /Roll_inj e; case: (Polyf_inj e)=> -> ->.
+- by move=> [<- <-].
+apply/(iffP andP).
+- case=> [/eqP -> e]; split=> //.
+  elim: {i_y yargs xargs} (nth_fin i_y).2 x y e=> [[] []|n IH] //=.
+  by case=> [[/= x Px] xs] [y ys] /= /andP [/Px -> /IH ->].
+- case=> [-> <-]; split=> //.
+  elim: {i_y y yargs xargs} (nth_fin i_y).2 x=> [[]|n IH] //=.
+  case=> [[/= x Px] xs]; apply/andP; split; [exact/Px|exact/IH].
 Qed.
 
 Definition CoqIndEqMixin := EqMixin ind_eqP.
@@ -721,21 +757,21 @@ End GenericEqType.
 
 Section Instances.
 
-Variables (A : Type) (A_sort : A -> Type).
-Local Coercion A_sort : A >-> Sortclass.
-Variables (a a1 a2 : A).
+Import CoqInd.
 
-Definition unit_signature : signature A := [:: [::]].
+Variables (a a1 a2 : Type).
+
+Definition unit_signature : signature := [:: [::]].
 
 Definition unit_constructors :
-  CoqInd.constructors A_sort unit unit_signature := (tt, tt).
+  CoqInd.constructors unit unit_signature := (tt, tt).
 
 Definition unit_rec :
-  CoqInd.recursor A_sort unit unit_signature :=
+  CoqInd.recursor unit unit_signature :=
   fun S => @unit_rect (fun _ => S).
 
 Definition unit_case :
-  CoqInd.destructor A_sort unit unit_signature :=
+  CoqInd.destructor unit unit_signature :=
   fun S ftt x => match x with tt => ftt end.
 
 Lemma unit_recE :
@@ -751,19 +787,19 @@ Proof. exact: unit_rect. Qed.
 
 Definition unit_coqIndMixin := CoqIndMixin unit_recE unit_caseE unit_indP.
 Canonical unit_coqIndType :=
-  Eval hnf in CoqIndType _ _ _ unit unit_coqIndMixin.
+  Eval hnf in CoqIndType _ unit unit_coqIndMixin.
 
-Definition void_signature : signature A := [::].
+Definition void_signature : signature := [::].
 
 Definition void_constructors :
-  CoqInd.constructors A_sort void void_signature := tt.
+  CoqInd.constructors void void_signature := tt.
 
 Definition void_rec :
-  CoqInd.recursor A_sort void void_signature :=
+  CoqInd.recursor void void_signature :=
   fun S => @Empty_set_rect (fun _ => S).
 
 Definition void_case :
-  CoqInd.destructor A_sort void void_signature :=
+  CoqInd.destructor void void_signature :=
   fun S x => match x with end.
 
 Lemma void_recE :
@@ -779,20 +815,20 @@ Proof. exact: Empty_set_rect. Qed.
 
 Definition void_coqIndMixin := CoqIndMixin void_recE void_caseE void_indP.
 Canonical void_coqIndType :=
-  Eval hnf in CoqIndType _ _ _ void void_coqIndMixin.
+  Eval hnf in CoqIndType _ void void_coqIndMixin.
 
-Definition bool_signature : signature A := [:: [::]; [::]].
+Definition bool_signature : signature := [:: [::]; [::]].
 
 Definition bool_constructors :
-  CoqInd.constructors A_sort bool bool_signature :=
+  CoqInd.constructors bool bool_signature :=
   (true, (false, tt)).
 
 Definition bool_rec :
-  CoqInd.recursor A_sort bool bool_signature :=
+  CoqInd.recursor bool bool_signature :=
   fun S => @bool_rect (fun _ => S).
 
 Definition bool_case :
-  CoqInd.destructor A_sort bool bool_signature :=
+  CoqInd.destructor bool bool_signature :=
   fun S ftrue ffalse b => if b then ftrue else ffalse.
 
 Lemma bool_recE : CoqInd.recursor_eq bool_constructors bool_rec.
@@ -806,18 +842,18 @@ Proof. exact: bool_rect. Qed.
 
 Definition bool_coqIndMixin := CoqIndMixin bool_recE bool_caseE bool_indP.
 Canonical bool_coqIndType :=
-  Eval hnf in CoqIndType A A_sort _ bool bool_coqIndMixin.
+  Eval hnf in CoqIndType _ bool bool_coqIndMixin.
 
-Definition nat_signature : signature A := [:: [::]; [:: Rec]].
+Definition nat_signature : signature := [:: [::]; [:: Rec]].
 
 Definition nat_constructors :
-  CoqInd.constructors A_sort nat nat_signature :=
+  CoqInd.constructors nat nat_signature :=
   (O, (S, tt)).
 
-Definition nat_rec : CoqInd.recursor A_sort nat nat_signature :=
+Definition nat_rec : CoqInd.recursor nat nat_signature :=
   fun S => @nat_rect (fun _ => S).
 
-Definition nat_case : CoqInd.destructor A_sort nat nat_signature :=
+Definition nat_case : CoqInd.destructor nat nat_signature :=
   fun S fz fs n => if n is n.+1 then fs n else fz.
 
 Lemma nat_recE : CoqInd.recursor_eq nat_constructors nat_rec.
@@ -830,21 +866,21 @@ Lemma nat_indP P : CoqInd.ind_at P nat_constructors.
 Proof. exact: nat_rect. Qed.
 
 Definition nat_coqIndMixin := CoqIndMixin nat_recE nat_caseE nat_indP.
-Canonical nat_coqIndType := CoqIndType A A_sort _ nat nat_coqIndMixin.
+Canonical nat_coqIndType := CoqIndType _ nat nat_coqIndMixin.
 
-Definition option_signature : signature A :=
+Definition option_signature : signature :=
   [:: [:: Other a]; [::]].
 
 Definition option_constructors :
-  CoqInd.constructors A_sort (option a) option_signature :=
+  CoqInd.constructors (option a) option_signature :=
   (@Some a, (@None a, tt)).
 
 Definition option_rec :
-  CoqInd.recursor A_sort (option a) option_signature :=
+  CoqInd.recursor (option a) option_signature :=
   fun S => @option_rect a (fun _ => S).
 
 Definition option_case :
-  CoqInd.destructor A_sort (option a) option_signature :=
+  CoqInd.destructor (option a) option_signature :=
   fun S fsome fnone o =>
     if o is Some x then fsome x else fnone.
 
@@ -862,21 +898,21 @@ Proof. exact: option_rect. Qed.
 Definition option_coqIndMixin :=
   CoqIndMixin option_recE option_caseE option_indP.
 Canonical option_coqIndType :=
-  Eval hnf in CoqIndType _ _ _ (option a) option_coqIndMixin.
+  Eval hnf in CoqIndType _ (option a) option_coqIndMixin.
 
-Definition sum_signature : signature A :=
+Definition sum_signature : signature :=
   [:: [:: Other a1]; [:: Other a2]].
 
 Definition sum_constructors :
-  CoqInd.constructors A_sort (a1 + a2)%type sum_signature :=
+  CoqInd.constructors (a1 + a2)%type sum_signature :=
   (@inl _ _, (@inr _ _, tt)).
 
 Definition sum_rec :
-  CoqInd.recursor A_sort (a1 + a2)%type sum_signature :=
+  CoqInd.recursor (a1 + a2)%type sum_signature :=
   fun S => @sum_rect _ _ (fun _ => S).
 
 Definition sum_case :
-  CoqInd.destructor A_sort (a1 + a2)%type sum_signature :=
+  CoqInd.destructor (a1 + a2)%type sum_signature :=
   fun S finl finr x =>
     match x with inl x => finl x | inr x => finr x end.
 
@@ -890,21 +926,21 @@ Lemma sum_indP P : CoqInd.ind_at P sum_constructors.
 Proof. exact: sum_rect. Qed.
 
 Definition sum_coqIndMixin := CoqIndMixin sum_recE sum_caseE sum_indP.
-Canonical sum_coqIndType := Eval hnf in CoqIndType _ _ _ (a1 + a2)%type sum_coqIndMixin.
+Canonical sum_coqIndType := Eval hnf in CoqIndType _ (a1 + a2)%type sum_coqIndMixin.
 
-Definition prod_signature : signature A :=
+Definition prod_signature : signature :=
   [:: [:: Other a1; Other a2]].
 
 Definition prod_constructors :
-  CoqInd.constructors A_sort (a1 * a2)%type prod_signature :=
+  CoqInd.constructors (a1 * a2)%type prod_signature :=
   (@pair _ _, tt).
 
 Definition prod_rec :
-  CoqInd.recursor A_sort (a1 * a2)%type prod_signature :=
+  CoqInd.recursor (a1 * a2)%type prod_signature :=
   fun S => @prod_rect _ _ (fun _ => S).
 
 Definition prod_case :
-  CoqInd.destructor A_sort (a1 *  a2)%type prod_signature :=
+  CoqInd.destructor (a1 *  a2)%type prod_signature :=
   fun S c p => let: (x, y) := p in c x y.
 
 Lemma prod_recE : CoqInd.recursor_eq prod_constructors prod_rec.
@@ -918,21 +954,21 @@ Proof. exact: prod_rect. Qed.
 
 Definition prod_coqIndMixin := CoqIndMixin prod_recE prod_caseE prod_indP.
 Canonical prod_coqIndType :=
-  Eval hnf in CoqIndType _ _ _ (a1 * a2)%type prod_coqIndMixin.
+  Eval hnf in CoqIndType _ (a1 * a2)%type prod_coqIndMixin.
 
-Definition seq_signature : signature A :=
+Definition seq_signature : signature :=
   [:: [::]; [:: Other a; Rec]].
 
 Definition seq_constructors :
-  CoqInd.constructors A_sort (seq a) seq_signature :=
+  CoqInd.constructors (seq a) seq_signature :=
   (@nil _, (@cons _, tt)).
 
 Definition seq_rec :
-  CoqInd.recursor A_sort (seq a) seq_signature :=
+  CoqInd.recursor (seq a) seq_signature :=
   fun S => @list_rect _ (fun _ => S).
 
 Definition seq_case :
-  CoqInd.destructor A_sort (seq a) seq_signature :=
+  CoqInd.destructor (seq a) seq_signature :=
   fun S fnil fcons l =>
     match l with nil => fnil | cons x y => fcons x y end.
 
@@ -947,6 +983,6 @@ Proof. exact: list_rect. Qed.
 
 Definition seq_coqIndMixin := CoqIndMixin seq_recE seq_caseE seq_indP.
 Canonical seq_coqIndType :=
-  Eval hnf in CoqIndType _ _ _ (seq a) seq_coqIndMixin.
+  Eval hnf in CoqIndType _ (seq a) seq_coqIndMixin.
 
 End Instances.
